---
Layout: post
mathjax: true
comments: true
title:  "Shifted Gaussians and Hermite functions"
categories: Mathematics
date:   2014-04-15
---

**April 15, 2014.** *I give a simple method for calculating moments of a
  shifted Gaussian using the generating function for Hermite polynomials.*

The Hermite polynomials $H_n(\xi), n \in \mathbb{Z}_{\geq 0}$, are a classical family of orthogonal polynomials. In physics, they are most famous as the wavefunctions of the quantum harmonic oscillator. Hermite polynomials are often defined as derivatives, 

$$ 
H_n(\xi) := (-1)^ne^{\xi^2}\frac{d^n}{d\xi^n}e^{-\xi^2}, 
$$
 
but are more elegantly given as coefficients of a <i>generating function</i>, 

$$ 
\exp(2s\xi - s^2) = \sum_{n\geq 0}H_n(\xi)\frac{s^n}{n!}. 
$$
 
The generating function gives us a nice way to calculate integrals of products of Hermite polynomials. Since the Gaussian density $e^{-x^2}$ appears in both definitions, it's not surprising that the generating function turns up in the calculation of the "shifted" Gaussian integral 

$$ 
I_n(a, b) = \int_{-\infty}^\infty x^ne^{-ax^2 - bx}\,dx, \quad
        a \geq 0, \quad n \in \mathbb{Z}_{\geq0}. 
$$
 
Going through the details is a nice expos√© of the generating function method. 
 
The main trick is to assemble the $I_n$ terms into a power series.
 Define $C = (\pi/a)^{1/2} e^{b^2/4a}$, and consider 

$$ 
\begin{align*}
  \int_{-\infty}^\infty C^{-1}e^{tx}e^{-ax^2 - bx}\,dx & = \int_{-\infty}^\infty C^{-1}\sum_{n=0}^\infty \frac{t^nx^n}{n!}e^{-ax^2 - bx}\,dx \label{first}\\
          & = \sum_{n=0}^\infty \frac{t^n}{Cn!}\int_{-\infty}^\infty x^ne^{-ax^2 - bx}\,dx \notag\\
          & = \sum_{n=0}^\infty \frac{t^n}{Cn!}I_n(a, b). \end{align*} 
$$
 
We can evaluate the first expression directly using the standard
Gaussian integral $\,I_0(a, b-t)$:

$$
\begin{align*} 
\int_{-\infty}^\infty C^{-1}e^{tx}e^{-ax^2 - bx}\,dx
           & = C^{-1}\int_{-\infty}^\infty e^{-ax^2 - (b - t)x}\,dx \notag\\
           & =  \sqrt{\frac{a}{\pi}}e^{-b^2/4a} \cdot  \sqrt{\frac{\pi}{a}}e^{(b - t)^2/4a} \\ & = e^{(-b^2 + b^2 - 2bt + t^2)/4a}\\ &  = e^{(t^2 - 2bt)/4a}. 
		   \end{align*}
$$

 We observe that this is <i>almost</i> the Hermite generating function $e^{2s\xi - s^2}$.
 To massage it into that form, we change variables: 

$$ 
s = \frac{it}{2\sqrt{a}}, \quad \xi  = -\frac{bt}{4as} = \frac{ib}{2\sqrt{a}}. 
$$
 
 Using the Hermite polynomials,
 we have

$$
\begin{align*} 
e^{(t^2 - 2bt)/4a} &  = e^{2s\xi - s^2}\notag\\
  & = \sum_{n=0}^\infty \frac{H_n(\xi)}{n!}s^n \notag\\
  & = \sum_{n=0}^\infty \frac{1}{n!}\left(\frac{it}{2\sqrt{a}}\right)^nH_n\left(\frac{ib}{2\sqrt{a}}\right) \notag\\
  & = \sum_{n=0}^\infty
                \frac{i^nt^n}{n!2^na^{n/2}}H_n\left(\frac{ib}{2\sqrt{a}}\right). 
				\end{align*}
$$
				
 We now have two different power series for the same thing. Identifying them term by term gives
 us our rather neat final result:

$$
\begin{align*} 
% \frac{1}{Cn!}I_n(a,b) & = \frac{i^n}{n!2^na^{n/2}}H_n\left(\frac{ib}{2\sqrt{a}}\right) \\\implies \quad 
 I_n(a,b) & =
        e^{b^2/4a}\left(\frac{i}{2}\right)^n\sqrt{\frac{\pi}{a^{n+1}}}H_n\left(\frac{ib}{2\sqrt{a}}\right). 
		\end{align*}
$$

As a quick application, let's find the even moments of the Gaussian distribution: 

$$ 
I_{2n}(1, 0) = \int_{-\infty}^{\infty} x^{2n}e^{-x^2}\,dx. 
$$
 
 To evaluate this, we'll need the constant term of $H_{2n}$.
 We can use the generating function to get this too:

$$
\begin{align*} 
\sum_{n\geq 0}H_n(0)\frac{s^n}{n!} = \exp(-s^2) 
& = \sum_{k\geq 0}\frac{(-1)^ks^{2k}}{k!}. 
\end{align*}
$$

Hence, $H_{2n+1}(0) = 0$ and 

$$ 
H_{2n}(0) = \frac{(-1)^n(2n)!}{n!}. 
$$
 
Subbing in to our expression for $I_{2n}(1, 0)$, we get 

$$ 
\int_{-\infty}^{\infty} x^{2n}e^{-x^2}\,dx = \frac{(2n!)\sqrt{\pi}}{4^nn!}. 
$$
